cryptis/core/term/with_stdpp.v
@@ -261,7 +261,7 @@ Fixpoint val_of_term_rec t : val :=
   | TPair t1 t2 =>
     (#TOp2_tag, (#TPair_tag, val_of_term_rec t1, val_of_term_rec t2))%V
   | TNonce l =>
-    (#TOp0_tag, (#TNonce_tag, #l))%V
+    (#TOp0_tag, (#TNonce_tag, #(nonce_loc l)))%V
   | TKey kt t =>
     (#TOp1_tag, ((#TKey_tag, repr kt), val_of_term_rec t))%V
   | TSeal t1 t2 =>
@@ -334,7 +334,7 @@ Lemma nonces_of_termE' t :
   match t with
   | TInt _ => ∅
   | TPair t1 t2 => nonces_of_term t1 ∪ nonces_of_term t2
-  | TNonce l => {[l]}
+  | TNonce l => {[nonce_loc l]}
   | TKey _ t => nonces_of_term t
   | TSeal t1 t2 => nonces_of_term t1 ∪ nonces_of_term t2
   | THash t => nonces_of_term t
@@ -723,6 +723,9 @@ split.
       apply: (STMul (proj1 (is_trueP _) wf) sub' t'_ts).
 Qed.
 
+Lemma nonce_loc_inj : forall x y : nonce, nonce_loc x = nonce_loc y -> x = y.
+Proof. by move=> [x] [y] /= ->. Qed.
+
 Ltac solve_nonces_of_termP :=
   intros;
   repeat match goal with
@@ -730,6 +733,7 @@ Ltac solve_nonces_of_termP :=
       rewrite [nonces_of_term (X Y)]nonces_of_termE /= in H
   | H : _ ∈ {[_]} |- _ =>
       rewrite elem_of_singleton in H;
+      apply nonce_loc_inj in H;
       rewrite {}H
   | H : _ ∈ _ ∪ _ |- _ =>
       rewrite elem_of_union in H;
@@ -742,7 +746,7 @@ Ltac solve_nonces_of_termP :=
   end;
   eauto using subterm.
 
-Lemma nonces_of_termP a t : subterm (TNonce a) t ↔ a ∈ nonces_of_term t.
+Lemma nonces_of_termP (a : nonce) t : subterm (TNonce a) t ↔ nonce_loc a ∈ nonces_of_term t.
 Proof.
 split.
 - elim: t /; try by intros; rewrite nonces_of_termE; set_solver.
